<?xml version="1.0"?>
<rdf:RDF xmlns="https://w3id.org/mint/modelCatalog#"
     xml:base="https://w3id.org/mint/modelCatalog"
     xmlns:dc="http://purl.org/dc/elements/1.1/"
     xmlns:owl="http://www.w3.org/2002/07/owl#"
     xmlns:rdf="http://www.w3.org/1999/02/22-rdf-syntax-ns#"
     xmlns:xml="http://www.w3.org/XML/1998/namespace"
     xmlns:xsd="http://www.w3.org/2001/XMLSchema#"
     xmlns:rdfs="http://www.w3.org/2000/01/rdf-schema#"
     xmlns:vann="http://purl.org/vocab/vann/"
     xmlns:terms="http://purl.org/dc/terms/">
    <owl:Ontology rdf:about="https://w3id.org/mint/modelCatalog">
        <owl:versionIRI rdf:resource="https://w3id.org/mint/modelCatalog/0.3.0"/>
        <dc:abstract xml:lang="en">An ontology for describing models and their linkages to variables.</dc:abstract>
        <dc:contributor xml:lang="en">Jay Pujara</dc:contributor>
        <dc:contributor xml:lang="en">Lucas Carvalho</dc:contributor>
        <dc:creator xml:lang="en">Daniel Garijo</dc:creator>
        <dc:creator xml:lang="en">Varun Ratnakar</dc:creator>
        <dc:creator xml:lang="en">Yolanda Gil</dc:creator>
        <dc:creator>Deborah Khider</dc:creator>
        <dc:title xml:lang="en">The MINT Model Catalog Ontology</dc:title>
        <terms:license rdf:resource="http://creativecommons.org/licenses/by/2.0/"/>
        <vann:preferredNamespacePrefix xml:lang="en">https://w3id.org/mint/modelCatalog#</vann:preferredNamespacePrefix>
        <vann:preferredNamespacePrefix xml:lang="en">mc</vann:preferredNamespacePrefix>
        <vann:preferredNamespaceURI rdf:resource="https://w3id.org/mint/modelCatalog#"/>
        <rdfs:comment xml:lang="en">An ontology for describing models and their linkages to variables.</rdfs:comment>
        <owl:priorVersion rdf:resource="https://w3id.org/mint/modelCatalog/0.2.0"/>
        <owl:versionInfo>0.3.0</owl:versionInfo>
    </owl:Ontology>
    


    <!-- 
    ///////////////////////////////////////////////////////////////////////////////////////
    //
    // Annotation properties
    //
    ///////////////////////////////////////////////////////////////////////////////////////
     -->


    


    <!-- http://purl.org/dc/elements/1.1/contributor -->


    <owl:AnnotationProperty rdf:about="http://purl.org/dc/elements/1.1/contributor"/>
    


    <!-- http://purl.org/dc/elements/1.1/creator -->


    <owl:AnnotationProperty rdf:about="http://purl.org/dc/elements/1.1/creator"/>
    


    <!-- http://purl.org/dc/elements/1.1/license -->


    <owl:AnnotationProperty rdf:about="http://purl.org/dc/elements/1.1/license"/>
    


    <!-- http://purl.org/dc/elements/1.1/title -->


    <owl:AnnotationProperty rdf:about="http://purl.org/dc/elements/1.1/title"/>
    


    <!-- http://purl.org/vocab/vann/preferredNamespacePrefix -->


    <owl:AnnotationProperty rdf:about="http://purl.org/vocab/vann/preferredNamespacePrefix"/>
    


    <!-- http://purl.org/vocab/vann/preferredNamespaceUri -->


    <owl:AnnotationProperty rdf:about="http://purl.org/vocab/vann/preferredNamespaceUri"/>
    


    <!-- http://www.w3.org/2002/07/owl#priorVersion -->


    <owl:AnnotationProperty rdf:about="http://www.w3.org/2002/07/owl#priorVersion"/>
    


    <!-- 
    ///////////////////////////////////////////////////////////////////////////////////////
    //
    // Object Properties
    //
    ///////////////////////////////////////////////////////////////////////////////////////
     -->


    


    <!-- http://ontosoft.org/software#hasContainer -->


    <owl:ObjectProperty rdf:about="http://ontosoft.org/software#hasContainer">
        <rdfs:domain rdf:resource="http://ontosoft.org/software#Function"/>
        <rdfs:range rdf:resource="http://ontosoft.org/software#Container"/>
        <rdfs:comment xml:lang="en">Function to link a function with its corresponding container</rdfs:comment>
    </owl:ObjectProperty>
    


    <!-- http://ontosoft.org/software#hasSoftwareVersion -->


    <owl:ObjectProperty rdf:about="http://ontosoft.org/software#hasSoftwareVersion">
        <rdfs:domain rdf:resource="http://ontosoft.org/software#Software"/>
        <rdfs:range rdf:resource="http://ontosoft.org/software#SoftwareVersion"/>
        <rdfs:isDefinedBy rdf:resource="http://ontosoft.org/software#"/>
        <rdfs:label xml:lang="en">has software version</rdfs:label>
    </owl:ObjectProperty>
    


    <!-- https://w3id.org/mint/modelCatalog#hadGrid -->


    <owl:ObjectProperty rdf:about="https://w3id.org/mint/modelCatalog#hadGrid">
        <rdfs:domain>
            <owl:Class>
                <owl:unionOf rdf:parseType="Collection">
                    <rdf:Description rdf:about="https://w3id.org/mint/dataCatalog#Dataset"/>
                    <rdf:Description rdf:about="https://w3id.org/mint/modelCatalog#DatasetSpecification"/>
                </owl:unionOf>
            </owl:Class>
        </rdfs:domain>
        <rdfs:range rdf:resource="https://w3id.org/mint/modelCatalog#Grid"/>
        <rdfs:comment xml:lang="en">Links the variable presentation to its grid</rdfs:comment>
        <rdfs:label xml:lang="en">has grid</rdfs:label>
    </owl:ObjectProperty>
    


    <!-- https://w3id.org/mint/modelCatalog#hasCAG -->


    <owl:ObjectProperty rdf:about="https://w3id.org/mint/modelCatalog#hasCAG">
        <rdfs:domain rdf:resource="https://w3id.org/mint/modelCatalog#ModelConfiguration"/>
        <rdfs:range rdf:resource="https://w3id.org/mint/modelCatalog#CAG"/>
        <rdfs:comment xml:lang="en">Relates a model configuration to its CAG</rdfs:comment>
        <rdfs:label xml:lang="en">has CAG</rdfs:label>
    </owl:ObjectProperty>
    


    <!-- https://w3id.org/mint/modelCatalog#hasConfiguration -->


    <owl:ObjectProperty rdf:about="https://w3id.org/mint/modelCatalog#hasConfiguration">
        <rdfs:domain rdf:resource="https://w3id.org/mint/modelCatalog#ModelVersion"/>
        <rdfs:range rdf:resource="https://w3id.org/mint/modelCatalog#ModelConfiguration"/>
        <rdfs:comment xml:lang="en">Property that links a model to one of its configurations. A model may have multiple configurations, each of which is unique in terms of the inputs and outputs it uses.</rdfs:comment>
        <rdfs:label xml:lang="en">has configuration</rdfs:label>
    </owl:ObjectProperty>
    


    <!-- https://w3id.org/mint/modelCatalog#hasDataset -->


    <owl:ObjectProperty rdf:about="https://w3id.org/mint/modelCatalog#hasDataset">
        <owl:inverseOf rdf:resource="https://w3id.org/mint/modelCatalog#hasPresentation"/>
        <rdfs:domain rdf:resource="https://w3id.org/mint/modelCatalog#VariablePresentation"/>
        <rdfs:range>
            <owl:Class>
                <owl:unionOf rdf:parseType="Collection">
                    <rdf:Description rdf:about="https://w3id.org/mint/dataCatalog#Dataset"/>
                    <rdf:Description rdf:about="https://w3id.org/mint/modelCatalog#DatasetSpecification"/>
                </owl:unionOf>
            </owl:Class>
        </rdfs:range>
        <rdfs:comment xml:lang="en">Associates a presentation with a dataset where the presentation occurs</rdfs:comment>
        <rdfs:label xml:lang="en">has dataset</rdfs:label>
    </owl:ObjectProperty>
    


    <!-- https://w3id.org/mint/modelCatalog#hasFileStructure -->


    <owl:ObjectProperty rdf:about="https://w3id.org/mint/modelCatalog#hasFileStructure">
        <rdfs:domain rdf:resource="https://w3id.org/mint/modelCatalog#DatasetSpecification"/>
        <rdfs:range rdf:resource="https://w3id.org/mint/modelCatalog#DataStructureDefinition"/>
        <rdfs:comment xml:lang="en">Relates a dataset specification to the data structure definition</rdfs:comment>
        <rdfs:label xml:lang="en">has file structure</rdfs:label>
    </owl:ObjectProperty>
    


    <!-- https://w3id.org/mint/modelCatalog#hasInput -->


    <owl:ObjectProperty rdf:about="https://w3id.org/mint/modelCatalog#hasInput">
        <rdfs:domain rdf:resource="https://w3id.org/mint/modelCatalog#ModelConfiguration"/>
        <rdfs:range rdf:resource="https://w3id.org/mint/modelCatalog#DatasetSpecification"/>
        <rdfs:comment xml:lang="en">Property that links a model configuration to the input types expected by it.</rdfs:comment>
        <rdfs:label xml:lang="en">has input</rdfs:label>
    </owl:ObjectProperty>
    


    <!-- https://w3id.org/mint/modelCatalog#hasModule -->


    <owl:ObjectProperty rdf:about="https://w3id.org/mint/modelCatalog#hasModule">
        <rdfs:domain rdf:resource="https://w3id.org/mint/modelCatalog#ModelConfiguration"/>
        <rdfs:range rdf:resource="https://w3id.org/mint/modelCatalog#Module"/>
        <rdfs:comment xml:lang="en">link between a model configuration and a module being used on it</rdfs:comment>
        <rdfs:label xml:lang="en">has module</rdfs:label>
    </owl:ObjectProperty>
    


    <!-- https://w3id.org/mint/modelCatalog#hasOutput -->


    <owl:ObjectProperty rdf:about="https://w3id.org/mint/modelCatalog#hasOutput">
        <rdfs:domain rdf:resource="https://w3id.org/mint/modelCatalog#ModelConfiguration"/>
        <rdfs:range rdf:resource="https://w3id.org/mint/modelCatalog#DatasetSpecification"/>
        <rdfs:comment xml:lang="en">Preoperty that expresses what are the outputs of a model</rdfs:comment>
        <rdfs:label xml:lang="en">has output</rdfs:label>
    </owl:ObjectProperty>
    


    <!-- https://w3id.org/mint/modelCatalog#hasParameter -->


    <owl:ObjectProperty rdf:about="https://w3id.org/mint/modelCatalog#hasParameter">
        <rdfs:domain rdf:resource="https://w3id.org/mint/modelCatalog#ModelConfiguration"/>
        <rdfs:range rdf:resource="https://w3id.org/mint/modelCatalog#Parameter"/>
        <rdfs:comment xml:lang="en">Property that indicates the parameters of a model configuration</rdfs:comment>
        <rdfs:label xml:lang="en">has parameter</rdfs:label>
    </owl:ObjectProperty>
    


    <!-- https://w3id.org/mint/modelCatalog#hasPart -->


    <owl:ObjectProperty rdf:about="https://w3id.org/mint/modelCatalog#hasPart">
        <rdfs:domain rdf:resource="https://w3id.org/mint/modelCatalog#CAG"/>
        <rdfs:range rdf:resource="https://w3id.org/mint/modelCatalog#Process"/>
        <rdfs:comment xml:lang="en">Relates the CAG to the process</rdfs:comment>
        <rdfs:label xml:lang="en">has part</rdfs:label>
    </owl:ObjectProperty>
    


    <!-- https://w3id.org/mint/modelCatalog#hasPresentation -->


    <owl:ObjectProperty rdf:about="https://w3id.org/mint/modelCatalog#hasPresentation">
        <rdfs:domain>
            <owl:Class>
                <owl:unionOf rdf:parseType="Collection">
                    <rdf:Description rdf:about="https://w3id.org/mint/dataCatalog#Dataset"/>
                    <rdf:Description rdf:about="https://w3id.org/mint/modelCatalog#DatasetSpecification"/>
                </owl:unionOf>
            </owl:Class>
        </rdfs:domain>
        <rdfs:range rdf:resource="https://w3id.org/mint/modelCatalog#VariablePresentation"/>
        <rdfs:comment xml:lang="en">Property that links an instance of a dataset (or a dataset specification) to the presentation of a variable contained (or expected to be contained) on it.</rdfs:comment>
        <rdfs:label xml:lang="en">has presentation</rdfs:label>
    </owl:ObjectProperty>
    


    <!-- https://w3id.org/mint/modelCatalog#hasProcess -->


    <owl:ObjectProperty rdf:about="https://w3id.org/mint/modelCatalog#hasProcess">
        <rdfs:domain rdf:resource="https://w3id.org/mint/modelCatalog#ModelConfiguration"/>
        <rdfs:range rdf:resource="https://w3id.org/mint/modelCatalog#Process"/>
        <rdfs:comment xml:lang="en">Relates the model configuration to the processes being simulated.</rdfs:comment>
        <rdfs:label xml:lang="en">has process</rdfs:label>
    </owl:ObjectProperty>
    


    <!-- https://w3id.org/mint/modelCatalog#hasStandardVariable -->


    <owl:ObjectProperty rdf:about="https://w3id.org/mint/modelCatalog#hasStandardVariable">
        <rdfs:domain rdf:resource="https://w3id.org/mint/modelCatalog#VariablePresentation"/>
        <rdfs:range rdf:resource="https://w3id.org/mint/modelCatalog#StandardVariable"/>
        <rdfs:comment xml:lang="en">the standard name of a variable</rdfs:comment>
        <rdfs:label xml:lang="en">has standard variable</rdfs:label>
    </owl:ObjectProperty>
    


    <!-- https://w3id.org/mint/modelCatalog#hasTimeInterval -->


    <owl:ObjectProperty rdf:about="https://w3id.org/mint/modelCatalog#hasTimeInterval">
        <rdfs:domain rdf:resource="https://w3id.org/mint/modelCatalog#ModelConfiguration"/>
        <rdfs:range rdf:resource="https://w3id.org/mint/modelCatalog#TimeInterval"/>
        <rdfs:comment xml:lang="en">Property that relates the model configuration to the time interval on which it&apos;s being run.</rdfs:comment>
        <rdfs:label xml:lang="en">has time interval</rdfs:label>
    </owl:ObjectProperty>
    


    <!-- https://w3id.org/mint/modelCatalog#influences -->


    <owl:ObjectProperty rdf:about="https://w3id.org/mint/modelCatalog#influences">
        <rdfs:domain rdf:resource="https://w3id.org/mint/modelCatalog#Process"/>
        <rdfs:range rdf:resource="https://w3id.org/mint/modelCatalog#Process"/>
        <rdfs:comment xml:lang="en">Describe the realationship between two processes</rdfs:comment>
        <rdfs:label xml:lang="en">influences</rdfs:label>
    </owl:ObjectProperty>
    


    <!-- https://w3id.org/mint/modelCatalog#usesUnit -->


    <owl:ObjectProperty rdf:about="https://w3id.org/mint/modelCatalog#usesUnit">
        <rdfs:domain>
            <owl:Class>
                <owl:unionOf rdf:parseType="Collection">
                    <rdf:Description rdf:about="https://w3id.org/mint/modelCatalog#TimeInterval"/>
                    <rdf:Description rdf:about="https://w3id.org/mint/modelCatalog#VariablePresentation"/>
                </owl:unionOf>
            </owl:Class>
        </rdfs:domain>
        <rdfs:range rdf:resource="http://qudt.org/schema/qudt/Unit"/>
        <rdfs:comment xml:lang="en">Property used to link a variable presentation or time interval to the unit they are represented in</rdfs:comment>
        <rdfs:label xml:lang="en">Uses unit</rdfs:label>
    </owl:ObjectProperty>
    


    <!-- 
    ///////////////////////////////////////////////////////////////////////////////////////
    //
    // Data properties
    //
    ///////////////////////////////////////////////////////////////////////////////////////
     -->


    


    <!-- http://ontosoft.org/software#hasDocumentation -->


    <owl:DatatypeProperty rdf:about="http://ontosoft.org/software#hasDocumentation">
        <rdfs:comment xml:lang="en">Pointer to the documentation of the model</rdfs:comment>
        <rdfs:isDefinedBy rdf:resource="http://ontosoft.org/software#"/>
    </owl:DatatypeProperty>
    


    <!-- http://ontosoft.org/software#hasExecutionCommand -->


    <owl:DatatypeProperty rdf:about="http://ontosoft.org/software#hasExecutionCommand">
        <rdfs:domain rdf:resource="http://ontosoft.org/software#Container"/>
        <rdfs:range rdf:resource="http://www.w3.org/2001/XMLSchema#string"/>
        <rdfs:comment xml:lang="en">Execution instructions on how to run the image</rdfs:comment>
        <rdfs:label xml:lang="en">has execution command</rdfs:label>
    </owl:DatatypeProperty>
    


    <!-- http://ontosoft.org/software#hasIdentifier -->


    <owl:DatatypeProperty rdf:about="http://ontosoft.org/software#hasIdentifier">
        <rdfs:domain rdf:resource="http://ontosoft.org/software#Container"/>
        <rdfs:range rdf:resource="http://www.w3.org/2001/XMLSchema#string"/>
        <rdfs:comment xml:lang="en">Container id</rdfs:comment>
        <rdfs:label xml:lang="en">has container</rdfs:label>
    </owl:DatatypeProperty>
    


    <!-- http://ontosoft.org/software#hasImplementationScriptLocation -->


    <owl:DatatypeProperty rdf:about="http://ontosoft.org/software#hasImplementationScriptLocation">
        <rdfs:domain rdf:resource="http://ontosoft.org/software#Function"/>
        <rdfs:range rdf:resource="http://www.w3.org/2001/XMLSchema#anyURI"/>
        <rdfs:comment xml:lang="en">Property that points to the main runnable script for the current function</rdfs:comment>
        <rdfs:label xml:lang="en">has implementation script location</rdfs:label>
    </owl:DatatypeProperty>
    


    <!-- http://ontosoft.org/software#hasInstallationInstructions -->


    <owl:DatatypeProperty rdf:about="http://ontosoft.org/software#hasInstallationInstructions">
        <rdfs:domain rdf:resource="http://ontosoft.org/software#Container"/>
        <rdfs:range rdf:resource="http://www.w3.org/2001/XMLSchema#string"/>
        <rdfs:label xml:lang="en">has installation instructions</rdfs:label>
    </owl:DatatypeProperty>
    


    <!-- http://ontosoft.org/software#hasVersionId -->


    <owl:DatatypeProperty rdf:about="http://ontosoft.org/software#hasVersionId">
        <rdfs:domain rdf:resource="http://ontosoft.org/software#SoftwareVersion"/>
        <rdfs:range rdf:resource="http://www.w3.org/2001/XMLSchema#string"/>
        <rdfs:isDefinedBy rdf:resource="http://ontosoft.org/software#"/>
        <rdfs:label xml:lang="en">has version id</rdfs:label>
    </owl:DatatypeProperty>
    


    <!-- http://purl.org/dc/terms/description -->


    <owl:DatatypeProperty rdf:about="http://purl.org/dc/terms/description">
        <rdfs:isDefinedBy rdf:resource="http://purl.org/dc/terms/"/>
    </owl:DatatypeProperty>
    


    <!-- https://w3id.org/mint/modelCatalog#hasAssumption -->


    <owl:DatatypeProperty rdf:about="https://w3id.org/mint/modelCatalog#hasAssumption">
        <rdfs:domain>
            <owl:Class>
                <owl:unionOf rdf:parseType="Collection">
                    <rdf:Description rdf:about="https://w3id.org/mint/modelCatalog#Model"/>
                    <rdf:Description rdf:about="https://w3id.org/mint/modelCatalog#ModelConfiguration"/>
                </owl:unionOf>
            </owl:Class>
        </rdfs:domain>
        <rdfs:range rdf:resource="http://www.w3.org/2001/XMLSchema#string"/>
        <rdfs:comment xml:lang="en">Assumptions of a model, e.g. the solver being used.</rdfs:comment>
        <rdfs:label xml:lang="en">has assumption</rdfs:label>
    </owl:DatatypeProperty>
    


    <!-- https://w3id.org/mint/modelCatalog#hasComponentLocation -->


    <owl:DatatypeProperty rdf:about="https://w3id.org/mint/modelCatalog#hasComponentLocation">
        <rdfs:domain rdf:resource="http://ontosoft.org/software#Function"/>
        <rdfs:range rdf:resource="http://www.w3.org/2001/XMLSchema#anyURI"/>
        <rdfs:comment xml:lang="en">Location of the aggregation of all the files needed to execute the component. Usually a zip file including the run script and support scripts</rdfs:comment>
        <rdfs:comment xml:lang="en">has component location</rdfs:comment>
    </owl:DatatypeProperty>
    


    <!-- https://w3id.org/mint/modelCatalog#hasDataType -->


    <owl:DatatypeProperty rdf:about="https://w3id.org/mint/modelCatalog#hasDataType">
        <rdfs:domain rdf:resource="https://w3id.org/mint/modelCatalog#Parameter"/>
        <rdfs:range rdf:resource="http://www.w3.org/2001/XMLSchema#string"/>
        <rdfs:comment xml:lang="en">Property that indicates the data type of a parameter</rdfs:comment>
        <rdfs:label xml:lang="en">has data type</rdfs:label>
    </owl:DatatypeProperty>
    


    <!-- https://w3id.org/mint/modelCatalog#hasDefaultValue -->


    <owl:DatatypeProperty rdf:about="https://w3id.org/mint/modelCatalog#hasDefaultValue">
        <rdfs:domain>
            <owl:Class>
                <owl:unionOf rdf:parseType="Collection">
                    <rdf:Description rdf:about="https://w3id.org/mint/modelCatalog#Parameter"/>
                    <rdf:Description rdf:about="https://w3id.org/mint/modelCatalog#VariablePresentation"/>
                </owl:unionOf>
            </owl:Class>
        </rdfs:domain>
        <rdfs:range rdf:resource="http://www.w3.org/2001/XMLSchema#float"/>
        <rdfs:comment xml:lang="en">Default accepted value of a variable presentation (or a parameter)</rdfs:comment>
        <rdfs:label xml:lang="en">has default value</rdfs:label>
    </owl:DatatypeProperty>
    


    <!-- https://w3id.org/mint/modelCatalog#hasDimensionality -->


    <owl:DatatypeProperty rdf:about="https://w3id.org/mint/modelCatalog#hasDimensionality">
        <rdfs:domain rdf:resource="https://w3id.org/mint/modelCatalog#DatasetSpecification"/>
        <rdfs:range rdf:resource="http://www.w3.org/2001/XMLSchema#int"/>
        <rdfs:comment xml:lang="en">Property to indicate dimensionality of the input or output of a dataset specification</rdfs:comment>
        <rdfs:label xml:lang="en">has dimensionality</rdfs:label>
    </owl:DatatypeProperty>
    


    <!-- https://w3id.org/mint/modelCatalog#hasFormat -->


    <owl:DatatypeProperty rdf:about="https://w3id.org/mint/modelCatalog#hasFormat">
        <rdfs:domain rdf:resource="https://w3id.org/mint/modelCatalog#DatasetSpecification"/>
        <rdfs:range rdf:resource="http://www.w3.org/2001/XMLSchema#string"/>
        <rdfs:comment xml:lang="en">Format followed by a file. For example, txt, nc, etc.</rdfs:comment>
        <rdfs:label xml:lang="en">has format</rdfs:label>
    </owl:DatatypeProperty>
    


    <!-- https://w3id.org/mint/modelCatalog#hasLongName -->


    <owl:DatatypeProperty rdf:about="https://w3id.org/mint/modelCatalog#hasLongName">
        <rdfs:domain rdf:resource="https://w3id.org/mint/modelCatalog#VariablePresentation"/>
        <rdfs:range rdf:resource="http://www.w3.org/2001/XMLSchema#string"/>
        <rdfs:comment xml:lang="en">Properties that relate the variable representation to its long name. The long name is useful for context (e.g., precipitation is less ambiguous than P) but not as precise as the standard name.</rdfs:comment>
        <rdfs:label xml:lang="en">has long name</rdfs:label>
    </owl:DatatypeProperty>
    


    <!-- https://w3id.org/mint/modelCatalog#hasMaximumAcceptedValue -->


    <owl:DatatypeProperty rdf:about="https://w3id.org/mint/modelCatalog#hasMaximumAcceptedValue">
        <rdfs:domain>
            <owl:Class>
                <owl:unionOf rdf:parseType="Collection">
                    <rdf:Description rdf:about="https://w3id.org/mint/modelCatalog#Parameter"/>
                    <rdf:Description rdf:about="https://w3id.org/mint/modelCatalog#VariablePresentation"/>
                </owl:unionOf>
            </owl:Class>
        </rdfs:domain>
        <rdfs:range rdf:resource="http://www.w3.org/2001/XMLSchema#float"/>
        <rdfs:comment xml:lang="en">Maximum accepted value of a variable presentation (or a parameter)</rdfs:comment>
        <rdfs:label xml:lang="en">has maximum accepted value</rdfs:label>
    </owl:DatatypeProperty>
    


    <!-- https://w3id.org/mint/modelCatalog#hasMinimumAcceptedValue -->


    <owl:DatatypeProperty rdf:about="https://w3id.org/mint/modelCatalog#hasMinimumAcceptedValue">
        <rdfs:domain>
            <owl:Class>
                <owl:unionOf rdf:parseType="Collection">
                    <rdf:Description rdf:about="https://w3id.org/mint/modelCatalog#Parameter"/>
                    <rdf:Description rdf:about="https://w3id.org/mint/modelCatalog#VariablePresentation"/>
                </owl:unionOf>
            </owl:Class>
        </rdfs:domain>
        <rdfs:range rdf:resource="http://www.w3.org/2001/XMLSchema#float"/>
        <rdfs:comment xml:lang="en">Minimum accepted value of a variable presentation (or a parameter)</rdfs:comment>
        <rdfs:label xml:lang="en">has minimum accepted value</rdfs:label>
    </owl:DatatypeProperty>
    


    <!-- https://w3id.org/mint/modelCatalog#hasModelCategory -->


    <owl:DatatypeProperty rdf:about="https://w3id.org/mint/modelCatalog#hasModelCategory">
        <rdfs:domain rdf:resource="https://w3id.org/mint/modelCatalog#Model"/>
        <rdfs:range rdf:resource="http://www.w3.org/2001/XMLSchema#string"/>
        <rdfs:comment xml:lang="en">Realates a model to its category. For instance, Topoflow has category hydrology. Useful to quickly retrieve relevant models.</rdfs:comment>
        <rdfs:label xml:lang="en">has model category</rdfs:label>
    </owl:DatatypeProperty>
    


    <!-- https://w3id.org/mint/modelCatalog#hasRule -->


    <owl:DatatypeProperty rdf:about="https://w3id.org/mint/modelCatalog#hasRule">
        <rdfs:domain rdf:resource="https://w3id.org/mint/modelCatalog#ModelConfiguration"/>
        <rdfs:range rdf:resource="http://www.w3.org/2001/XMLSchema#string"/>
        <rdfs:comment xml:lang="en">Rule associated to the component</rdfs:comment>
        <rdfs:label xml:lang="en">has rule</rdfs:label>
    </owl:DatatypeProperty>
    


    <!-- https://w3id.org/mint/modelCatalog#hasShortName -->


    <owl:DatatypeProperty rdf:about="https://w3id.org/mint/modelCatalog#hasShortName">
        <rdfs:domain rdf:resource="https://w3id.org/mint/modelCatalog#VariablePresentation"/>
        <rdfs:range rdf:resource="http://www.w3.org/2001/XMLSchema#string"/>
        <rdfs:comment xml:lang="en">A short name (e.g., temperature) capturing the high-level concept of the variable</rdfs:comment>
        <rdfs:label xml:lang="en">has short name</rdfs:label>
    </owl:DatatypeProperty>
    


    <!-- https://w3id.org/mint/modelCatalog#hasSupportScriptLocation -->


    <owl:DatatypeProperty rdf:about="https://w3id.org/mint/modelCatalog#hasSupportScriptLocation">
        <rdfs:domain rdf:resource="http://ontosoft.org/software#Function"/>
        <rdfs:range rdf:resource="http://www.w3.org/2001/XMLSchema#anyURI"/>
        <rdfs:comment xml:lang="en">Property that links to the location of scripts that may be used from the main runnable script.</rdfs:comment>
        <rdfs:label xml:lang="en">has support script location</rdfs:label>
    </owl:DatatypeProperty>
    


    <!-- https://w3id.org/mint/modelCatalog#hasValue -->


    <owl:DatatypeProperty rdf:about="https://w3id.org/mint/modelCatalog#hasValue">
        <rdfs:domain rdf:resource="https://w3id.org/mint/modelCatalog#TimeInterval"/>
        <rdfs:range rdf:resource="http://www.w3.org/2001/XMLSchema#float"/>
        <rdfs:comment xml:lang="en">The numerical value associated with the object.</rdfs:comment>
        <rdfs:label xml:lang="en">has value</rdfs:label>
    </owl:DatatypeProperty>
    


    <!-- 
    ///////////////////////////////////////////////////////////////////////////////////////
    //
    // Classes
    //
    ///////////////////////////////////////////////////////////////////////////////////////
     -->


    


    <!-- http://ontosoft.org/software#Container -->


    <owl:Class rdf:about="http://ontosoft.org/software#Container"/>
    


    <!-- http://ontosoft.org/software#Function -->


    <owl:Class rdf:about="http://ontosoft.org/software#Function">
        <rdfs:comment rdf:datatype="http://www.w3.org/2001/XMLSchema#anyURI">&quot;Function&quot; is part of an Ontosoft extension currently being developed</rdfs:comment>
        <rdfs:isDefinedBy rdf:datatype="http://www.w3.org/2001/XMLSchema#anyURI">http://ontosoft.org/software#</rdfs:isDefinedBy>
    </owl:Class>
    


    <!-- http://ontosoft.org/software#Software -->


    <owl:Class rdf:about="http://ontosoft.org/software#Software">
        <rdfs:isDefinedBy rdf:datatype="http://www.w3.org/2001/XMLSchema#anyURI">http://ontosoft.org/software#</rdfs:isDefinedBy>
    </owl:Class>
    


    <!-- http://ontosoft.org/software#SoftwareVersion -->


    <owl:Class rdf:about="http://ontosoft.org/software#SoftwareVersion">
        <rdfs:isDefinedBy rdf:datatype="http://www.w3.org/2001/XMLSchema#anyURI">http://ontosoft.org/software#</rdfs:isDefinedBy>
    </owl:Class>
    


    <!-- http://qudt.org/schema/qudt/Unit -->


    <owl:Class rdf:about="http://qudt.org/schema/qudt/Unit">
        <rdfs:isDefinedBy rdf:resource="http://qudt.org/schema/qudt/"/>
    </owl:Class>
    


    <!-- http://schema.org/Dataset -->


    <owl:Class rdf:about="http://schema.org/Dataset"/>
    


    <!-- http://schema.org/Place -->


    <owl:Class rdf:about="http://schema.org/Place">
        <rdfs:isDefinedBy xml:lang="en">http://schema.org</rdfs:isDefinedBy>
    </owl:Class>
    


    <!-- http://www.geoscienceontology.org/geo-upper#Variable -->


    <owl:Class rdf:about="http://www.geoscienceontology.org/geo-upper#Variable">
        <owl:equivalentClass rdf:resource="https://w3id.org/mint/modelCatalog#GSNVariable"/>
        <rdfs:isDefinedBy rdf:resource="http://www.geoscienceontology.org/geo-upper"/>
    </owl:Class>
    


    <!-- http://www.w3.org/2004/02/skos/core#Concept -->


    <owl:Class rdf:about="http://www.w3.org/2004/02/skos/core#Concept">
        <rdfs:isDefinedBy rdf:resource="http://www.w3.org/2004/02/skos/core"/>
    </owl:Class>
    


    <!-- http://www.w3.org/ns/dcat#Dataset -->


    <owl:Class rdf:about="http://www.w3.org/ns/dcat#Dataset"/>
    


    <!-- https://w3id.org/mint/dataCatalog#Dataset -->


    <owl:Class rdf:about="https://w3id.org/mint/dataCatalog#Dataset">
        <rdfs:subClassOf rdf:resource="http://schema.org/Dataset"/>
        <rdfs:subClassOf rdf:resource="http://www.w3.org/ns/dcat#Dataset"/>
        <rdfs:comment xml:lang="en">Extension of the W3C Data Catalog dataset that has additional properties for the MINT data catalog</rdfs:comment>
        <rdfs:label xml:lang="en">Dataset</rdfs:label>
    </owl:Class>
    


    <!-- https://w3id.org/mint/modelCatalog#CAG -->


    <owl:Class rdf:about="https://w3id.org/mint/modelCatalog#CAG">
        <rdfs:comment>Causal analysis graph describing the processes being modeled and the relationship among them</rdfs:comment>
        <rdfs:label xml:lang="en">Causal analysis graph</rdfs:label>
    </owl:Class>
    


    <!-- https://w3id.org/mint/modelCatalog#DataStructureDefinition -->


    <owl:Class rdf:about="https://w3id.org/mint/modelCatalog#DataStructureDefinition">
        <rdfs:comment xml:lang="en">The schema the file follows. To make the input or output machin readable, we need to know how the file is organized.</rdfs:comment>
        <rdfs:label xml:lang="en">Data structure definition</rdfs:label>
    </owl:Class>
    


    <!-- https://w3id.org/mint/modelCatalog#DatasetSpecification -->


    <owl:Class rdf:about="https://w3id.org/mint/modelCatalog#DatasetSpecification">
        <rdfs:comment xml:lang="en">Class designed to describe a type of input or output used or produced by a model. For example, Topoflow has several inputs. One of them is a text file with precipitation values. The representation of this input is an instance of a dataset specification.</rdfs:comment>
        <rdfs:label xml:lang="en">Dataset specification</rdfs:label>
    </owl:Class>
    


    <!-- https://w3id.org/mint/modelCatalog#GSNVariable -->


    <owl:Class rdf:about="https://w3id.org/mint/modelCatalog#GSNVariable">
        <rdfs:subClassOf rdf:resource="https://w3id.org/mint/modelCatalog#StandardVariable"/>
        <rdfs:comment xml:lang="en">Variable that follows the GSN standard: http://geoscienceontology.org/</rdfs:comment>
        <rdfs:label xml:lang="en">GSN variable</rdfs:label>
    </owl:Class>
    


    <!-- https://w3id.org/mint/modelCatalog#Grid -->


    <owl:Class rdf:about="https://w3id.org/mint/modelCatalog#Grid">
        <rdfs:comment xml:lang="en">Datasets are often regridded before a simulation. Describes the grid convention being followed</rdfs:comment>
        <rdfs:label xml:lang="en">Grid</rdfs:label>
    </owl:Class>
    


    <!-- https://w3id.org/mint/modelCatalog#ICASAVariable -->


    <owl:Class rdf:about="https://w3id.org/mint/modelCatalog#ICASAVariable">
        <rdfs:subClassOf rdf:resource="https://w3id.org/mint/modelCatalog#StandardVariable"/>
        <rdfs:comment xml:lang="en">Variable that follows the ICASA standard for agriculture: https://dssat.net/data/standards_v2</rdfs:comment>
        <rdfs:label xml:lang="en">ICASA variable</rdfs:label>
    </owl:Class>
    


    <!-- https://w3id.org/mint/modelCatalog#Model -->


    <owl:Class rdf:about="https://w3id.org/mint/modelCatalog#Model">
        <rdfs:subClassOf rdf:resource="http://ontosoft.org/software#Software"/>
        <rdfs:comment xml:lang="en">A scientific model (from Hydrology, Agronomy, etc.) that represents a set of processes (infiltration, outflow, etc.) to be simulated.</rdfs:comment>
        <rdfs:label xml:lang="en">Model</rdfs:label>
    </owl:Class>
    


    <!-- https://w3id.org/mint/modelCatalog#ModelConfiguration -->


    <owl:Class rdf:about="https://w3id.org/mint/modelCatalog#ModelConfiguration">
        <rdfs:subClassOf rdf:resource="http://ontosoft.org/software#Function"/>
        <rdfs:comment xml:lang="en">A model may be configured in different ways depending on the data that is avaialble. For example, if topological information is available,  a groundwater model may use it to produce a better estimation of the water budget of an aquifer. A model configuration represents a unique setting of inputs and outputs of a given model designed for a particular functionality.</rdfs:comment>
        <rdfs:label xml:lang="en">Model configuration</rdfs:label>
    </owl:Class>
    


    <!-- https://w3id.org/mint/modelCatalog#ModelVersion -->


    <owl:Class rdf:about="https://w3id.org/mint/modelCatalog#ModelVersion">
        <rdfs:subClassOf rdf:resource="http://ontosoft.org/software#SoftwareVersion"/>
        <rdfs:comment xml:lang="en">The version of the model</rdfs:comment>
        <rdfs:label xml:lang="en">Model Version</rdfs:label>
    </owl:Class>
    


    <!-- https://w3id.org/mint/modelCatalog#Module -->


    <owl:Class rdf:about="https://w3id.org/mint/modelCatalog#Module">
        <rdfs:comment xml:lang="en">A module is an optional software package that can be configured to run in a model configuration.</rdfs:comment>
        <rdfs:label xml:lang="en">Module</rdfs:label>
    </owl:Class>
    


    <!-- https://w3id.org/mint/modelCatalog#Parameter -->


    <owl:Class rdf:about="https://w3id.org/mint/modelCatalog#Parameter">
        <rdfs:comment xml:lang="en">A parameter of the model.</rdfs:comment>
        <rdfs:label xml:lang="en">Parameter</rdfs:label>
    </owl:Class>
    


    <!-- https://w3id.org/mint/modelCatalog#Process -->


    <owl:Class rdf:about="https://w3id.org/mint/modelCatalog#Process">
        <rdfs:comment xml:lang="en">The biophysical or socio-economical behavior the model is simulating.</rdfs:comment>
        <rdfs:label xml:lang="en">Process</rdfs:label>
    </owl:Class>
    


    <!-- https://w3id.org/mint/modelCatalog#StandardVariable -->


    <owl:Class rdf:about="https://w3id.org/mint/modelCatalog#StandardVariable">
        <rdfs:subClassOf rdf:resource="https://w3id.org/mint/modelCatalog#Variable"/>
        <rdfs:comment xml:lang="en">A standard variable, necessary to refer to all the variable using the same nomenclature in a domain ontology</rdfs:comment>
        <rdfs:label xml:lang="en">Standard variable</rdfs:label>
    </owl:Class>
    


    <!-- https://w3id.org/mint/modelCatalog#TimeInterval -->


    <owl:Class rdf:about="https://w3id.org/mint/modelCatalog#TimeInterval">
        <rdfs:comment xml:lang="en">The time step of the model.</rdfs:comment>
        <rdfs:label xml:lang="en">Time interval</rdfs:label>
    </owl:Class>
    


    <!-- https://w3id.org/mint/modelCatalog#Unit -->


    <owl:Class rdf:about="https://w3id.org/mint/modelCatalog#Unit">
        <rdfs:subClassOf rdf:resource="http://qudt.org/schema/qudt/Unit"/>
        <rdfs:comment xml:lang="en">Class designed to distinguish the different types of units that are available in variables from datasets</rdfs:comment>
        <rdfs:label xml:lang="en">Unit</rdfs:label>
    </owl:Class>
    


    <!-- https://w3id.org/mint/modelCatalog#Variable -->


    <owl:Class rdf:about="https://w3id.org/mint/modelCatalog#Variable">
        <rdfs:comment xml:lang="en">A symbol that represents a quanity in a dataset or dataset specification</rdfs:comment>
        <rdfs:label xml:lang="en">Variable</rdfs:label>
    </owl:Class>
    


    <!-- https://w3id.org/mint/modelCatalog#VariablePresentation -->


    <owl:Class rdf:about="https://w3id.org/mint/modelCatalog#VariablePresentation">
        <rdfs:subClassOf rdf:resource="https://w3id.org/mint/modelCatalog#Variable"/>
        <rdfs:comment xml:lang="en">Concept used to represent an instantiation of a variable in an input/output dataset. For example, a model A may use an input file with temperature expressed in Farenheit (variablePresentation1), while a model B may produce an output with temperature in Celsius (variablePresentation2). Both variable presentations refer to the concept of temperature.</rdfs:comment>
        <rdfs:label xml:lang="en">Variable presentation</rdfs:label>
    </owl:Class>
</rdf:RDF>



<!-- Generated by the OWL API (version 5.1.7) https://github.com/owlcs/owlapi/ -->


